% === Exercise 11.6.1 ===
\begin{Exercise}
\begin{enumerate}[a)]
\item
\begin{proof}
For any $(a,b)$, consider
$$
\begin{cases} 
3u-v=a & \\ 
2u+5v=b &
\end{cases}.
$$
Compute
$$ 
\Delta = \begin{vmatrix}
3 & -1\\ 
2 & 5
\end{vmatrix}
= 17 \text{ , }
\Delta u = \begin{vmatrix}
3 & a \\
2 & b
\end{vmatrix}
= 3b-2a \text{, and }
\Delta v = \begin{vmatrix}
a & -1 \\
b & 5
\end{vmatrix}
= 5a+b.
$$
Use Cramer's Rule, we know 
$$
u=\frac{3b-2a}{17}\text{ and } v=\frac{5a+b}{17}.
$$
Hence, $u$ and $v$ are well defined. Then $f^{-1}$ exists and is differentiable in some nonempty, open set containing $(a,b)$. Moreover,
$$
D f(u,v) = \begin{bmatrix}
3 & -1 \\
2 & 5
\end{bmatrix},
$$
by the Inverse Function Theorem with $f(u,v) = (a,b)$, then
$$D (f^{-1}) (a,b) = \left( D f(u,v) \right)^{-1} = \frac{1}{17}\begin{bmatrix}
5 & 1 \\
-2 & 3
\end{bmatrix}.
$$
\end{proof}

\item
\begin{proof}
Consider
\begin{alignat*}{7}
\quad&& &\begin{cases} 
u+v=0 \\ 
\sin u+\cos v=1
\end{cases} \\
\implies&& &\sin u +\cos u = 1 \\
\implies&& &\frac{\sqrt{2}}{2}\sin u +\frac{\sqrt{2}}{2}\cos u = \frac{\sqrt{2}}{2} \\
\implies&& &\cos\frac{\pi}{4}\sin u + \sin\frac{\pi}{4}\cos u = \sin\frac{\pi}{4} \\
\implies&& &\sin(u+\frac{\pi}{4}) = \sin\frac{\pi}{4} \\
\implies&& &u+\frac{\pi}{4} = 2k\pi + \frac{\pi}{4}\mathbf{\ or\ }u+\frac{\pi}{4} = \pi-\left( 2k\pi+\frac{\pi}{4} \right)
\end{alignat*}
for $k\in\mathbb{Z}$. Hence we have
$$
\begin{cases}
u=2k\pi \\
v=-2k\pi
\end{cases} \text{ or }
\begin{cases}
u=-2k\pi+\frac{\pi}{2} \\
v=2k\pi-\frac{\pi}{2}
\end{cases}.
$$
Now $u$ and $v$ are well defined. Then $f^{-1}$ exists and is differentiable in some nonempty, open set containing $(0,1)$. Moreover,
$$
D f(2k\pi,-2k\pi) = \begin{bmatrix}
1 & 1 \\
1 & 0
\end{bmatrix}\text{ and }
D f(-2k\pi+\frac{\pi}{2}, 2k\pi-\frac{\pi}{2}) = \begin{bmatrix}
1 & 1 \\
0 & 1
\end{bmatrix}.
$$
Apply the Inverse Function Theorem with $f(u,v) = (0,1)$, then
$$
D (f^{-1})(0,1) = \begin{bmatrix}
0 & 1 \\
1 & -1
\end{bmatrix}\text{ or }
\begin{bmatrix}
1 & -1 \\
0 & 1
\end{bmatrix}.
$$
\end{proof}
\end{enumerate}
\end{Exercise}