% === Exercise 6.2.1 ===
\begin{Exercise}
\begin{enumerate}[a)]
\item 
\begin{proof}
Let 
$$
a_n := \frac{2n+5}{3n^3+2n-1}\text{ and } b_n :=\frac{1}{n^2}.
$$

Since $\sum_{k=1}^{\infty}\frac{1}{k^2}$ converges by the p-Series Test; besides,
$$
0
< \lim_{n\to\infty}\frac{a_n}{b_n} 
= \frac{2}{3} 
< \infty.
$$

By the Limit Comparison Test, we conclude 
$$
\sum_{k=1}^{\infty}\frac{2k+5}{3k^3+2k-1}
$$ 
converges.
\end{proof}

\item [d)]
\begin{proof}
Since $\log{k} < k,\ \forall k \in \mathbb{N}$, we have 
$$
\sum_{k=1}^{\infty}\frac{k^3\log^2{k}}{e^k} 
\leq \sum_{k=1}^{\infty}\frac{k^5}{e^k}.
$$

Let 
$$
a_n := \frac{n^5}{e^n}\text{ and } b_n :=\frac{1}{n^2}.
$$

Since $\sum_{k=1}^{\infty}\frac{1}{k^2}$ converges by the p-Series Test; besides,
$$
\lim_{n\to\infty}\frac{a_n}{b_n} 
= \lim_{n\to\infty}\frac{n^7}{e^n} 
= 0. 
$$
By the Limit Comparison Test and the Comparison Test, we conclude 
$$
\sum_{k=1}^{\infty}\frac{k^3\log^2{k}}{e^k}
$$ 
converges.
\end{proof}
\end{enumerate}
\end{Exercise}