% === Exercise 11.4.5 ===
\begin{Exercise}
\begin{proof}
At first, we claim
$$
\frac{\partial u}{\partial r} = \frac{1}{r}\frac{\partial v}{\partial \theta}.
$$
Consider
$$
\frac{\partial u}{\partial r} = \frac{\partial f}{\partial x}\cos \theta + \frac{\partial f}{\partial y}\sin \theta,
$$
and
$$
\frac{\partial v}{\partial \theta} = \frac{\partial g}{\partial x}(-r\sin\theta) + \frac{\partial g}{\partial y}(r\cos \theta).
$$
By hypothesis that $f,g$ satisfy the Cauchy-Riemann equations, we have
\begin{align*}
\frac{\partial u}{\partial r}
&= \frac{\partial f}{\partial x}\cos \theta + \frac{\partial f}{\partial y}\sin \theta \\
&= \frac{\partial g}{\partial y}\cos \theta - \frac{\partial g}{\partial x}\sin \theta \\
&= \frac{1}{r}\left( \frac{\partial g}{\partial x}(-r\sin \theta) + \frac{\partial g}{\partial y}(r\sin \theta) \right) \\
&= \frac{1}{r}\frac{\partial v}{\partial \theta}.
\end{align*}

Secondly, we claim
$$
\frac{\partial v}{\partial r} = -\frac{1}{r}\frac{\partial u}{\partial \theta}.
$$
Consider
$$
\frac{\partial v}{\partial r} = \frac{\partial g}{\partial x}\cos \theta + \frac{\partial g}{\partial y}\sin \theta,
$$
and
$$
\frac{\partial u}{\partial \theta} = \frac{\partial f}{\partial x}(-r\sin\theta) + \frac{\partial f}{\partial y}(r\cos\theta).
$$
By hypothesis that $f,g$ satisfy the Cauchy-Riemann equations, we have
\begin{align*}
\frac{\partial v}{\partial r}
&= \frac{\partial g}{\partial x}\cos\theta + \frac{\partial g}{\partial y}(r\cos\theta) \\
&= -\frac{\partial f}{\partial y}\cos\theta + \frac{\partial f}{\partial x}\sin\theta \\
&= -\frac{1}{r}\left( \frac{\partial f}{\partial x}(-r\sin\theta) + \frac{\partial f}{\partial y}(r\cos\theta) \right) \\
&= -\frac{1}{r}\frac{\partial u}{\partial \theta}.
\end{align*}

We make two claims hold, hence we complete the proof.
\end{proof}
\end{Exercise}