% === Exercise 11.4.3 ===
\begin{Exercise}
\begin{proof}
Consider
$$
\quad \rho^k f(x) = f(\rho x).
$$
Since $f$ is differentiable on $\mathbb{R}^n$, we differentiate both sides in $\rho$, then
$$
k \rho^{k-1} f(x) 
= \nabla f(\rho x) \frac{\partial}{\partial \rho} \rho x
= \nabla f(\rho x)\cdot x.
$$
Since it holds for all $\rho\in\mathbb{R}$, we pick $\rho = 1$, then
$$
k f(x) = \nabla f(x)\cdot x
$$
which implies
$$
x_1\frac{\partial f}{\partial x_1}(x) + \cdots + x_n\frac{\partial f}{\partial x_n}(x) = k f(x)
$$
for all $x=(x_1,\cdots,x_n)\in\mathbb{R}^n$.
\end{proof}
\end{Exercise}