% === Exercise 11.4.4 ===
\begin{Exercise}
\begin{proof}
Consider
$$
\frac{\partial u}{\partial x} = y f'(x y)\text{ and }\frac{\partial u}{\partial y} = x f'(x y),
$$
we have
$$
x\frac{\partial u}{\partial x} - y\frac{\partial u}{\partial y} = 0.
$$

On the other hand,
\begin{align*}
\frac{\partial v}{\partial x} &= f'(x-y)+g'(x+y); \\
\frac{\partial^2 v}{\partial x^2} &= f''(x-y)+g''(x+y), \\
\frac{\partial v}{\partial y} &= -f'(x-y)+g'(x+y); \\
\frac{\partial^2 v}{\partial y^2} &= f''(x-y)+g''(x+y). \\
\end{align*}
Hence,
$$
\frac{\partial^2 v}{\partial x^2} - \frac{\partial^2 v}{\partial y^2} = 0.
$$
\end{proof}
\end{Exercise}