% === Exercise 6.4.3 ===
\begin{Exercise}
\begin{enumerate}[a)]
\item
\begin{solution}
Let 
$$
a_k := \frac{(-1)^k k^3}{(k+1)!}.
$$

Since 
$$
\lim_{k\to\infty}\left|\frac{a_{k+1}}{a_k}\right| 
= \lim_{k\to\infty}\left|\frac{-1}{k+2}\left(\frac{k+1}{k}\right)^3\right| 
= 0 
< 1,
$$ by the Ratio Test, we conclude the series \textbf{converges absolutely}.
\end{solution}

\item
\begin{solution}
Let 
$$a_k := \frac{(-1)\times(-3)\times...\times(1-2k)}{1 \times 4 \times ... \times (3k-2)}.
$$

Since 
$$
\lim_{k\to\infty}\left|\frac{a_{k+1}}{a_k}\right| 
= \lim_{k\to\infty}\left|\frac{-2k-1}{3k+1}\right| 
= \frac{2}{3} 
< 1,
$$ by the Ratio Test, we conclude the series \textbf{converges absolutely}.
\end{solution}

\item
\begin{solution}
Let 
$$
a_k := \frac{\left( k+1 \right)^k}{p^k k!}.
$$

Since 
$$
\lim_{k\to\infty}\left|\frac{a_{k+1}}{a_k}\right| 
= \lim_{k\to\infty}\left|\frac{k+2}{p\left(k+1\right)}\left(1+\frac{1}{k+1}\right)^k\right| 
= \frac{e}{p}
$$ 
where 
$$
\lim_{k\to\infty}\left(1+\frac{1}{k+1}\right)^k = e,
$$
by the Ratio Test, we conclude the series \textbf{converges absolutely}.
\end{solution}

\item
\begin{solution}
Let
$$
a_k := \frac{\sqrt{k}}{k+1}.
$$

Calculate 
$$
a_k' = \frac{-3k-1}{2\sqrt{k}\left(k+1\right)^2} < 0
$$ 
since $k\in\mathbb{N}$. Moreover, 
$$
\lim_{k\to\infty}a_k = 0,
$$ 
so we know 
$$
a_k\downarrow 0\text{ as }k\to\infty.
$$ 

By the Alternating Series Test, we have 
$$
\sum_{k=1}^{\infty}\left(-1\right)^{k+1}a_k
$$ 
which converges.

Is it absolutely convergent? Using the divergent p-Series
$$
b_k := \frac{1}{k},
$$ 
we have 
$$
\lim_{k\to\infty}\frac{a_k}{b_k}
= \lim_{k\to\infty}\left(\frac{\sqrt{k}}{1+\frac{1}{k}}\right) 
= \infty.
$$ 

By the Limit Comparison Test, we know 
$$
\sum_{k=1}^{\infty}a_k
$$ 
diverges. Then we conclude the series \textbf{converges conditionally}.
\end{solution}

\item
\begin{solution}
Let 
$$
a_k := \frac{(-1)^k\sqrt{k+1}}{\sqrt{k}\ k^k}.
$$

Since
$$
\lim_{k\to\infty}\left|\frac{a_{k+1}}{a_k}\right| 
= \lim_{k\to\infty}\left(\sqrt{\frac{k+2}{k+1}}\sqrt{\frac{k}{k+1}}\left(\frac{1}{k+1}\right)\left(1-\frac{1}{k+1}\right)^k\right) 
= 0 
< 1
$$
where 
$$
\lim_{k\to\infty}\left(1-\frac{1}{k+1}\right)^k 
= \frac{1}{e}.
$$

By the Ratio Test, we conclude the series \textbf{converges absolutely}.
\end{solution}
\end{enumerate}
\end{Exercise}