% === Exercise 6.4.6 ===
\begin{Exercise}
\begin{proof}
Let 
$$
B_{n,m} := \sum_{k=m}^{n}b_k.
$$

By Abel's formula, consider 
\begin{equation}\label{eq:abel}
\sum_{k=1}^{n}a_k b_k 
= B_{n,1}a_n + \sum_{k=1}^{n-1}B_{k,1}(a_k-a_{k+1}).
\end{equation}

Since $a_n\to 0$ as $n\to\infty$ and $B_{n,1}$ is bounded by the hypotheses, then 
$$
B_{n,1}a_n\to 0\text{ as }n\to\infty.
$$

On the other hand, 
$$
\sum_{k=1}^{n-1}\left|B_{k,1}(a_k-a_{k+1})\right| 
\leq M\sum_{k=1}^{n-1}\left|a_k-a_{k+1}\right|.
$$ 
Since 
$$
\sum_{k=1}^{\infty}\left|a_k-a_{k+1}\right| 
= \sum_{k=1}^{\infty}\left|a_{k+1}-a_k\right|
$$
converges by the hypotheses. By the Comparison Test, we know 
$$
\sum_{k=1}^{\infty}\left|B_{k,1}(a_k-a_{k+1})\right|
$$ 
converges so does
$$
\sum_{k=1}^{\infty}B_{k,1}(a_k-a_{k+1}).
$$

Finally, taking the limit of both sides on the equation \eqref{eq:abel}, we conclude
$$
\sum_{k=1}^{\infty}a_k b_k 
= \sum_{k=1}^{\infty}B_{k,1}(a_k-a_{k+1})
$$ 
converges as promised.
\end{proof}
\end{Exercise}