% === Exercise 6.4.5 ===
\begin{Exercise}
\begin{proof}
By Abel's formula, consider 
$$
\sum_{k=1}^{n}a_k b_k 
=  A_{n,1}b_n - \sum_{k=1}^{n-1}A_{k,1}(b_{k+1}-b_k)
= A_{n,1}b_n + \sum_{k=1}^{n-1}A_{k,1}(b_k-b_{k+1}).
$$ 

Notice $A_{n,1} = \sum_{k=1}^{n}a_k = s_n$ and $s_n$ is bounded by the hypotheses. 

Since $b_n\to 0\text{ as } n\to\infty$, then $s_n b_n\to 0\text{ as } n\to\infty$. Now taking the limit on both sides as $n\to\infty$, we conclude  
$$
\sum_{k=1}^{\infty}a_k b_k 
= \sum_{k=1}^{\infty}s_k (b_k - b_{k+1}).
$$
\end{proof}
\end{Exercise}