% === Exercise 11.5.6 ===
\begin{Exercise}
\begin{enumerate}[a)]
\item
\begin{solution}
\begin{align*}
g'(t)
&= \frac{\partial}{\partial x}f(t x+(1-t)a, y)\cdot\frac{\partial}{\partial t}(t x+(1-t)a) \\
&\quad +\frac{\partial}{\partial y}f(t x+(1-t)a,y)\cdot\frac{\partial}{\partial t}(y) \\
&\quad +\frac{\partial}{\partial x}f(a, t y+(1-t)b)\cdot\frac{\partial}{\partial t}(a) \\
&\quad +\frac{\partial}{\partial y}f(a, t y+(1-t)b)\cdot\frac{\partial}{\partial t}(t y+(1-t)b) \\
&= (x-a)\frac{\partial}{\partial x}f(t x+(1-t)a,y) + (y-b)\frac{\partial}{\partial y}f(a,t y+(1-t)b).
\end{align*}
\end{solution}

\item
\begin{proof}
By hypothesis which satisfy the Mean Value Theorem, there is $t\in(0,1)$ such that
$$
g(1)-g(0) = g'(t).
$$
which implies there are numbers $c=t x+(1-t)a$ and $d=t y+(1-t)b$ so that $c$ is between $a$ and $x$, and $d$ is between $b$ and $y$, such that
\begin{alignat*}{7}
\quad&& g(1)-g(0) &= g'(t) \\
\implies&& f(x,y)-f(a,b) &= (x-a)\frac{\partial}{\partial x}f(t x+(1-t)a,y) + (y-b)\frac{\partial}{\partial y}f(a,t y+(1-t)b) \\
\implies&& f(x,y)-f(a,b) &= (x-a)f_x(c,y)+(y-b)f_y(a,d).
\end{alignat*}
\end{proof}
\end{enumerate}
\end{Exercise}