% === Exercise 11.5.1 ===
\begin{Exercise}
\begin{enumerate}[a)]
\item
\begin{solution}
Notice that
\begin{alignat*}{5}
f_x &= 2x+y;&\quad f_y &= x+2y; &\quad &\quad\\
f_{x x} &= 2;&\quad f_{x y} &= f_{y x} = 1;&\quad f_{y y} &= 2.
\end{alignat*}

Use Theorem 11.37, by setting $a=(-1,1), h=(x+1,y-1)$, then
$$
f(x,y) = f(-1,1) + D^{(1)} f\left( (-1,1);(x+1,y-1)\right) + \frac{1}{2!} D^{(2)} f\left( (-1,1);(x+1,y-1) \right).
$$

Compute 
\begin{align*}
D^{(1)} f\left( (-1,1);(x+1,y-1)\right)
&= \nabla f(-1,1)\cdot(x+1,y-1) \\
&= -(x+1)+(y-1),
\end{align*}
and
\begin{align*}
D^{(2)} f\left( (-1,1);(x+1,y-1) \right)
&= (x+1)^2 f_{x x}(-1, 1) + (x+1)(y-1) f_{x y}(-1,1) + (y-1)^2 f_{y y}(-1,1) \\
&= 2(x+1)^2 + 2(x+1)(y-1) + 2(y-1)^2.
\end{align*}

Hence,
$$
f(x,y) = 1-(x+1)+(y-1)+(x+1)^2+(x+1)(y-1)+(y-1)^2.
$$
\end{solution}

\item [c)]
\begin{solution}
Notice that
\begin{alignat*}{7}
f_x &= y e^{x y}; &\quad f_y &= x e^{x y};\\
f_{x x} &= y^2 e^{x y}; &\quad f_{x y} &= (1+x y)e^{x y}; &\quad f_{y y} &= x^2 e^{x y}; \\
f_{x x x} &= y^3 e^{x y}; &\quad f_{x x y} &= (2y+x y^2)e^{x y}; &\quad f_{x y y} &= (2x+x^2 y)e^{x y}; \\
f_{y y y} &= x^3 e^{x y}; &\quad f_{x x x x} &= y^4 e^{x y}; &\quad f_{x x x y} &= (3y^2+x y^3)e^{x y}; \\
f_{x x y y} &= (2+4x y+x^2 y^2)e^{x y}; &\quad f_{x y y y} &= (2x^2+x^2+x^3 y)e^{x y}; &\quad f_{y y y y} &= x^4 e^{x y}.
\end{alignat*}

Use Theorem 11.37, there is $(c,d)\in L\left( (x,y); (0,0) \right)$ such that
$$
f(x,y) = f(0,0) + \sum_{k=1}^{3} D^{(k)} \frac{1}{k!} f\left( (0,0);(x,y)\right) + D^{(4)}\frac{1}{4!}f\left( (c,d);(x,y)\right).
$$
Computing patiently, we have
\begin{align*}
D^{(1)} f\left( (0,0);(x,y)\right) &= 0; \\
D^{(2)} f\left( (0,0);(x,y)\right) &= 2 x y; \\
D^{(3)} f\left( (0,0);(x,y)\right) &= 0; \\
D^{(4)} f\left( (c,d);(x,y)\right) 
&=  \left( (d x+c y)^4 + 12(d x+c y)^2 x y + 12x^2 y^2 \right) e^{c d}.\\
\end{align*}
Hence,
$$
e^{x y} = 1+x y + \frac{1}{4!} \left( (d x+c y)^4 + 12(d x+c y)^2 x y + 12x^2 y^2 \right) e^{c d}
$$
for some $(c,d)\in L\left( (x,y);(0,0) \right)$.
\end{solution}
\end{enumerate}
\end{Exercise}