% === Exercise 7.3.10 ===
\begin{Exercise}
\begin{proof}
Set 
$$
f(x) = \sum_{k=0}^{\infty}(-1)^k a_k x^k.
$$ 

For any $x\in[0,1]$, since $a_k \downarrow 0$ as $k\to\infty$, we know $f(x)$ converges on $[0,1]$ by the Alternating Series Test. 

Moreover, by the Abel's Theorem, $f(x)$ is continuous and converges uniformly on $[0,1]$; hence, given $\epsilon >0$, there is a $\delta>0$ such that $$\left| f(x) - f(y) \right| < \epsilon\mbox{, } \forall x,y\in[0,1].$$ which implies $$\left| \sum_{k=0}^{\infty}(-1)^k a_k (x^k - y^k) \right| < \epsilon.$$
\end{proof}
\end{Exercise}