% === Exercise 8.1.2 ===
\begin{Exercise}
\begin{enumerate}[a)]
\item 
\begin{proof}
Consider 
\begin{align*}
\|v\| 
&= \left\| \frac{(a\cdot b)c+(a\cdot c)b+(c\cdot b)a}{3} \right\| \\
&= \frac{1}{3} \left( \|a\cdot b\| \|c\| + \|a\cdot c\| \|b\|+\|c\cdot b\| \|a\|\right) \\
&\leq \|a\|\|b\| \|c\| \\
&\leq 1,
\end{align*}
hence $v\in B$ as promised.
\end{proof}

\item
\begin{proof}
For all $c, d\in \mathbb{R}^n$,
\begin{align*}
|a\cdot c - b\cdot d|
&= |a\cdot c - a\cdot b + a\cdot b - b\cdot d| \\
&= | a(c-b) + b(a-d) | \\
&\leq | a(c-b) | + | b(a-d) | \\
&= \|a\|\|b-c\| + \|b\|\|a-d\| \\
&\leq \|b-c\| + \|a-d\|
\end{align*}
\end{proof}

\item
\begin{proof}
\begin{align*}
\sqrt{|a\cdot (b \times c) |^2 + |a\cdot b|^2}
&= \sqrt{|(a \times b) \cdot c|^2 + |a\cdot b|^2} \\
&= \sqrt{\|a\times b\|^2 \|c\|^2 + |a\cdot b|^2} \\
&\leq \sqrt{\|a\times b\|^2 + |a\cdot b|^2} \\
&= \sqrt{(a\cdot a)(b\cdot b) - (a\cdot b)^2 + |a\cdot b|^2} \\
&= \sqrt{(\|a\|^2 \|b\|^2 - |a\cdot b|^2 + |a\cdot b|^2} \\
&= \sqrt{\|a\|^2 \|b\|^2} \\
&\leq 1
\end{align*}
\end{proof}
\end{enumerate}
\end{Exercise}