% === Exercise 11.1.5 ===
\begin{Exercise}
\begin{enumerate}[a)]
\item
\begin{solution}
Let $f(x,y) = e^{x^3y^2+x}$ and $f$ is continuous on $H=[0,1]\times[0,1]$. 

By Theorem 11.4, we know
$$
\lim_{y\to 0}\int_{0}^{1} e^{x^3y^2+x}\ dx
= \int_{0}^{1} \lim_{y\to 0} e^{x^3y^2+x}\ dx
= \int_{0}^{1} e^x\ dx
= e-1.
$$
\end{solution}

\item
\begin{solution}
Let $f(x,y) = \sin(e^x y-y^3+\pi-e^x)$ and $H = [0,1]\times[0,1]$.

For each $y\in[0,1]$, $f(\cdot,y)$ is continuous on $[0,1]$, and hence integrable.
We calculate $f_y(x,y) = \cos(\pi-1)(e^x-3)$, then $f_y(x,\cdot)$ exists on $[c,d]$, and $f_y(x,y)$ is continuous on $H$.

By Theorem 11.5, we have
\begin{align*}
\left. \frac{d}{dy} \right|_{y=1}\int_{0}^{1} \sin(e^x y-y^3+\pi-e^x)\ dx
&= \int_{0}^{1} \left. \frac{\partial f}{\partial y} \right|_{y=1} \sin(e^x y-y^3+\pi-e^x)\ dx \\
&= \int_{0}^{1} \left. \cos(e^x y-y^3+\pi-e^x)(e^x-3) \right|_{y=1} \ dx \\
&= \int_{0}^{1} \cos(\pi-1)(e^x-3)\ dx \\
&= \cos(\pi-1)(e-4).
\end{align*}
\end{solution}

\item
\begin{solution}
Let $f(x,y,z)=\sqrt{x^3+y^3+z^3-2}$ and $H = [1,3]\times[1,3]\times[1,3]$.

Since
\begin{align*}
f_x(x,y,z) &= \frac{3x^2}{2\sqrt{x^3+y^3+z^3-2}}; \\
f_y(x,y,z) &= \frac{3y^2}{2\sqrt{x^3+y^3+z^3-2}}; \\
f_z(x,y,z) &= \frac{3z^2}{2\sqrt{x^3+y^3+z^3-2}},
\end{align*}
we know $f\in C^{1}(H)$.

Therefore, by Theorem 11.5, we have
\begin{align*}
\left. \frac{\partial}{\partial x} \right|_{(x,y)=(1,1)} \int_{1}^{3} \sqrt{x^3+y^3+z^3-2}\ dz
&= \int_{1}^{3} \left. \frac{\partial}{\partial x}\right|_{(x,y)=(1,1)}\sqrt{x^3+y^3+z^3-2}\ dz \\
&= \int_{1}^{3} \left. \frac{3x^2}{2\sqrt{x^3+y^3+z^3-2} } \right|_{(x,y)=(1,1)}\ dz \\
&= \frac{3}{2} \int_{1}^{3} z^{-\frac{3}{2}}\ dz \\
&= -3 \left. z^{-\frac{1}{2}} \right|_{1}^{3} \\
&= 3-\sqrt{3}.
\end{align*}
\end{solution}
\end{enumerate}
\end{Exercise}