% === Exercise 6.3.6 ===
\begin{Exercise}
\begin{enumerate}[a)]
\item 
\begin{proof}
For $N\in\mathbb{N}$, $$ \sum_{k=1}^{\infty}\left( \sum_{j=1}^{N}a_{kj} \right) = \sum_{j=1}^{N}\left( \sum_{k=1}^{\infty}a_{kj} \right) $$ by the Limit Theorem. Then fix $N$, for any $K\in\mathbb{N}$, $$ \sum_{k=1}^{K}\left( \sum_{j=1}^{N}a_{kj} \right) \leq \sum_{k=1}^{\infty}\left( \sum_{j=1}^{\infty}a_{kj} \right).$$
If right hand side is finite, by the Monotone Convergence Theorem, we have $$\sum_{k=1}^{\infty}\left( \sum_{j=1}^{N}a_{kj} \right) \leq \sum_{k=1}^{\infty}\left( \sum_{j=1}^{\infty}a_{kj} \right).$$
On the other hand if it is infinite, then it holds trivially. Hence for any $N\in\mathbb{N}$, $$\sum_{j=1}^{N}\left( \sum_{k=1}^{\infty}a_{kj} \right) \leq \sum_{k=1}^{\infty}\left( \sum_{j=1}^{\infty}a_{kj} \right).$$ Using the Monotone Convergence Theorem again, we conclude $$\sum_{j=1}^{\infty}\left( \sum_{k=1}^{\infty}a_{kj} \right) \leq \sum_{k=1}^{\infty}\left( \sum_{j=1}^{\infty}a_{kj} \right).$$
\end{proof}

\item
\begin{proof}
Set $B_j = \sum_{k=1}^{\infty}a_{kj}$. From part a), $$ \sum_{j=1}^{\infty}B_j = \sum_{j=1}^{\infty}\left( \sum_{k=1}^{\infty}a_{kj} \right) \leq \sum_{k=1}^{\infty}\left( \sum_{j=1}^{\infty}a_{kj} \right) = \sum_{k=1}^{\infty}A_k$$ converges so does $\sum_{j=1}^{\infty}B_j$ which implies both $$\sum_{j=1}^{\infty}\left( \sum_{k=1}^{\infty}a_{kj} \right) \leq \sum_{k=1}^{\infty}\left( \sum_{j=1}^{\infty}a_{kj} \right) \mbox{ and } \sum_{k=1}^{\infty}\left( \sum_{j=1}^{\infty}a_{kj} \right) \leq \sum_{j=1}^{\infty}\left( \sum_{k=1}^{\infty}a_{kj} \right) $$ hold. So we conclude $$\sum_{j=1}^{\infty}\left( \sum_{k=1}^{\infty}a_{kj} \right) = \sum_{k=1}^{\infty}\left( \sum_{j=1}^{\infty}a_{kj} \right).$$
\end{proof}

\item
\begin{proof}
Consider $$a_{kj} = \begin{cases}1 & \mbox{if } j=k \\
-1 & \mbox{if }j=k+1 \\
0 & \mbox{otherwise} \end{cases}.$$
Then the equation from part b) implies $$ 1 = 0 $$ which is obviously a contradiction.
\end{proof}
\end{enumerate}
\end{Exercise}