% === Exercise 7.2.10 ===
\begin{Exercise}
\begin{proof}
Let $$g_n(x) := \left( \sum_{k=1}^{n} f_k^n(x) \right)^\frac{1}{n}.$$
Consider for all $x\in[a,b]$, since $0 \leq f_k(x) \leq f_{k+1}(x) \implies f_k^n(x) \leq f_{k+1}^{n}(x)$. 
Hence
$$g_n(x) \leq \left( nf_n^n(x) \right)^\frac{1}{n} = n^{\frac{1}{n}}f_n(x) \leq 2f_n(x)$$ for $n$ sufficiently large.
Notice $f_n\to f$ uniformly on $[a,b]$, hence $g_n$ converges uniformly on $[a,b]$.
We know given $\epsilon > 0$, $\exists N\in\mathbb{N}$ such that $$n\geq N \implies n^{\frac{1}{n}} < 1+\epsilon,$$ hence
\begin{alignat*}{7}
&& g_n(x) &\leq (1+\epsilon)f_n(x) \\
\implies&& \int_{a}^{b} g_n(x) d x &\leq (1+\epsilon)\int_{a}^{b}f_n(x) d x \\
\implies&& \lim_{n\to\infty} \int_{a}^{b} g_n(x) d x &\leq \lim_{n\to\infty}\left( (1+\epsilon)\int_{a}^{b}f_n(x) d x \right) \\
\quad&& &= (1+\epsilon)\int_{a}^{b}\lim_{n\to\infty}f_n(x) d x \\
\quad&& &= (1+\epsilon)\int_{a}^{b}f(x) d x
\end{alignat*}

This holds for any $\epsilon>0$, hence
\begin{equation}\label{eq:ex10.1}
\lim_{n\to\infty} \int_{a}^{b} g_n(x) d x \leq \int_{a}^{b} f(x) d x.
\end{equation}
On the other hand, since $f_{k+1}(x) \geq f_k(x) \geq 0$ on $[a,b]$,
\begin{align*}
g_n(x)
=& \left( \sum_{k=1}^{n} f_k^n(x) \right)^{\frac{1}{n}} \\
=& \left( \sum_{k=1}^{N-1}f_k^n(x) + \sum_{k=N}^{n}f_k^n(x) \right)^{\frac{1}{n}} \\
\geq& \left( \sum_{k=N}^{n}f_k^n(x) \right)^{\frac{1}{n}} \\
\geq& (n-N)^{\frac{1}{n}} f_N(x).
\end{align*}
Then, $$\int_{a}^{b} \left( \sum_{k=1}^{n} f_k^n(x) \right)^{\frac{1}{n}} dx \geq \int_{a}^{b} (n-N)^{\frac{1}{n}} f_N(x) dx.$$
Taking the limit of both sides as $n\to\infty$,
$$ \lim_{n\to\infty} \int_{a}^{b} \left( \sum_{k=1}^{n} f_k^n(x) \right)^{\frac{1}{n}} dx \geq \int_{a}^{b} f_N(x) dx.$$
Taking the limit of both sides as $N\to\infty$, 
\begin{equation}\label{eq:ex10.2}
\lim_{n\to\infty} \int_{a}^{b} \left( \sum_{k=1}^{n} f_k^n(x) \right)^{\frac{1}{n}} dx \geq \int_{a}^{b} f(x) dx.
\end{equation}
From equation \eqref{eq:ex10.1} and \eqref{eq:ex10.2}, we conclude $$
\lim_{n\to\infty} \int_{a}^{b} \left( \sum_{k=1}^{n} f_k^n(x) \right)^{\frac{1}{n}} dx = \int_{a}^{b} f(x) dx.$$
\end{proof}
\end{Exercise}