% === Exercise 7.2.7 ===
\begin{Exercise}
\begin{proof}
Since $g_1$ is bounded on $E$ and $g_k(x) \geq g_{k+1}(x) \geq 0$ for all $x\in E$ and $k\in\mathbb{N}$, we know there is a number $M>0$ such that $$\left| g_n(x) \right| \leq M$$ for all $x\in E$ and $n\in\mathbb{N}$.
Set $$S_n(x) := \sum_{k=1}^{n}f_k(x)\mbox{ and } S(x) := \sum_{k=1}^{\infty}f_k(x).$$
Since $f$ converges uniformly on $E$, given $\epsilon>0$, $\exists N\in\mathbb{N}$ such that $$n>m>N \implies \left| S_n(x)-S_{m-1}(x) \right| \leq \frac{\epsilon}{3M}\mbox{ and } \left| S_{m-1}(x)-S(x) \right| \leq \frac{\epsilon}{3M}.$$
Hence, 
\begin{align*}
&\quad \left| \sum_{k=m}^{n} f_k(x) g_k(x) \right| \\
&= \left| S_n(x) g_n(x) - S_{m-1} g_m(x) + \sum_{k=m}^{n-1}S_k(x)\left( g_k(x)-g_{k+1}(x) \right) \right| \\
&= \left| \left[ S_n(x)-S_{m-1}(x) \right] g_n(x) + S_{m-1}(x) \left[ g_n(x)-g_m(x) \right] + \sum_{k=m}^{n-1}S_k(x)\left( g_k(x)-g_{k+1}(x) \right) \right| \\
&\leq \left| \left( S_n(x)-S_{m-1}(x) \right) g_n(x) + \left( S_{m-1}(x)-S(x) \right) \left( g_n(x) - g_m(x) \right) \right| \\
&\quad + \left| \sum_{k=m}^{n-1}\left( S_k(x)-S(x) \right) \left( g_k(x)-g_{k+1}(x) \right) \right| \\
&< \frac{\epsilon}{3M} \times M + \frac{\epsilon}{3M} \times M + \frac{\epsilon}{3M} \times M \\
&= \epsilon.
\end{align*}
By the Uniform Cauchy Criterion, $\sum_{k=1}^{\infty}f_k g_k$ converges uniformly on $E$.
\end{proof}
\end{Exercise}